Wrong answer on test 1



```c++
#include <bits/stdc++.h>
using namespace std;
 
// Global variables per test case.
int n; // number of initial terms (1-indexed)
vector<long long> preA;       // preA[i] = a1 + a2 + ... + a_i
vector<int> preB;            // preB[i] = (preA[i] mod 2)
vector<long long> preB_prefix; // preB_prefix[i] = preB[1] + ... + preB[i]
int r0; // = preA[n] mod 2 (the parity of the total initial sum)
 
// We'll memoize two functions:
// F_B(x) = sum_{j=1}^{x} B(j) where for j<=n, B(j)=preB[j] and for j>n,
// B(j) is defined as: if (j odd) then r0, else r0 XOR B(j/2).
unordered_map<long long, long long> memoF;
// B(x): returns B(x)=A(x) mod 2.
unordered_map<long long, int> memoB;
 
// F_B(x): sum of B(j) for j=1..x.
long long F_B(long long x) {
    if(x <= 0) return 0;
    if(x <= n) return preB_prefix[x];
    if(memoF.count(x)) return memoF[x];
    long long base = preB_prefix[n]; // contribution for j=1..n
    long long total = x - n;         // number of j in [n+1, x]
    // Count odds in [n+1, x]:
    long long odds = ((x + 1) / 2) - ((n + 1) / 2);
    long long evens = total - odds;
    long long res = 0;
    if(r0 == 0) {
        // For j > n: odd j give 0; even j (j = 2*k) contribute B(2*k)=B(k).
        long long kL = (n + 1 + 1) / 2; // ceil((n+1)/2)
        long long kR = x / 2;           // floor(x/2)
        long long evenSum = 0;
        if(kR >= kL) evenSum = F_B(kR) - F_B(kL - 1);
        res = base + evenSum;
    } else { // r0 == 1
        // For j > n: odd j give 1; even j (j=2*k) give 1 XOR B(k) = 1 - B(k).
        long long kL = (n + 1 + 1) / 2;
        long long kR = x / 2;
        long long evenCount = 0, evenSum = 0;
        if(kR >= kL) {
            evenCount = (kR - kL + 1);
            long long sumB = F_B(kR) - F_B(kL - 1);
            evenSum = evenCount - sumB;
        }
        res = base + odds + evenSum;
    }
    memoF[x] = res;
    return res;
}
 
// S_B(L, R): sum of B(j) for j in [L, R].
long long S_B(long long L, long long R) {
    if(L > R) return 0;
    return F_B(R) - F_B(L - 1);
}
 
// B(x): returns B(x) = A(x) mod 2.
// For j <= n, B(x) = preB[x]. For j > n, if (x odd) then r0, else r0 XOR B(x/2).
int B_val(long long x) {
    if(x <= n) return preB[x];
    if(memoB.count(x)) return memoB[x];
    int res;
    if(x & 1LL) {
        res = r0;
    } else {
        res = r0 ^ B_val(x / 2);
    }
    memoB[x] = res;
    return res;
}
 
// G(x): for x > n, G(x) = sum_{m=n+1}^{x} a_m.
// Using the recurrence that for m>n, a_m = B_val(floor(m/2)),
// we group by j = floor(m/2). For each j such that m = 2*j or 2*j+1 lies in [n+1,x]:
//   - If x is even, let M = x/2. Then for j from j1 = ceil((n+1)/2) to M-1, each j gives 2*B_val(j)
//     and if M >= j1 then add B_val(M) (only m=2*M is included).
//   - If x is odd, let M = floor(x/2) and each j in [j1, M] contributes 2*B_val(j).
long long G_func(long long x) {
    long long M = x / 2; // floor(x/2)
    long long j1 = (n + 2) / 2; // ceil((n+1)/2)
    if(M < j1) return 0;
    long long ret = 0;
    if((x & 1LL) == 0) { // even x
        ret = 2 * S_B(j1, M - 1);
        ret += B_val(M);
    } else {
        ret = 2 * S_B(j1, M);
    }
    return ret;
}
 
// A(x): sum_{i=1}^{x} a_i. For x <= n, it's preA[x]. For x > n, A(x)= preA[n] + G(x).
long long A_func(long long x) {
    if(x <= 0) return 0;
    if(x <= n) return preA[x];
    return preA[n] + G_func(x);
}
 
// Main
int main(){
    ios::sync_with_stdio(false);
    cin.tie(nullptr);
 
    int t;
    cin >> t;
    while(t--){
        cin >> n;
        preA.resize(n+1);
        preB.resize(n+1);
        preB_prefix.resize(n+1);
        vector<int> arr(n+1);
 
        long long s = 0;
        for (int i = 1; i <= n; i++){
            cin >> arr[i];
            s += arr[i];
            preA[i] = s;
            preB[i] = preA[i] & 1;
        }
        preB_prefix[0] = 0;
        for (int i = 1; i <= n; i++){
            preB_prefix[i] = preB_prefix[i-1] + preB[i];
        }
 
        long long l, r;
        cin >> l >> r;
 
        r0 = preA[n] & 1;
 
        // Clear memoization maps for current test case.
        memoF.clear();
        memoB.clear();
 
        long long ans = A_func(r) - A_func(l - 1);
        cout << ans << "\n";
    }
    return 0;
}

```

